prove spi_read
prove trace property for SPI poll timeout

WIP

WIP xchg does not match...

WIP

WIP

WIP

WIP

WIP

WIP

WIP

WIP

WIP

WIP

WIP

tailrec_earlyout

WIP

WIP

WIP

recvEthernet passes again

WIP

WIP

WIP

prove iot_ok

print assumptions

bedrock2/src/Examples/LAN9250.v
@@ -16,34 +16,25 @@ Definition lan9250_readword : function :=
   let addr : varname := "addr" in
   let ret : varname := "ret" in
   let err : varname := "err" in
-  let SPI_CSMODE_ADDR := Ox"10024018" in
-  ("lan9250_readword", ((addr::nil), (ret::nil), bedrock_func_body:(
+  let SPI_CSMODE_ADDR := "SPI_CSMODE_ADDR" in
+  ("lan9250_readword", ((addr::nil), (ret::err::nil), bedrock_func_body:(
+    SPI_CSMODE_ADDR = (constr:(Ox"10024018"));
     io! ret = MMIOREAD(SPI_CSMODE_ADDR);
     ret = (ret | constr:(2));
     output! MMIOWRITE(SPI_CSMODE_ADDR, ret);
 
-    unpack! err = spi_write(constr:(Ox"0b"));        require !err; (* FASTREAD *)
-    unpack! err = spi_write(addr >> constr:(8));     require !err;
-    unpack! err = spi_write(addr & constr:(Ox"ff")); require !err;
-    unpack! err = spi_write(err);                    require !err; (* dummy *)
-    unpack! err = spi_write(err);                    require !err; (* read *)
-    unpack! err = spi_write(err);                    require !err; (* read *)
-    unpack! err = spi_write(err);                    require !err; (* read *)
-    unpack! err = spi_write(err);                    require !err; (* read *)
-
-    unpack! ret, err = spi_read(); require !err; (* write *)
-    unpack! ret, err = spi_read(); require !err; (* write *)
-    unpack! ret, err = spi_read(); require !err; (* write *)
-    unpack! ret, err = spi_read(); require !err; (* write *)
-
     (* manually register-allocated, apologies for variable reuse *)
-    unpack! ret, err = spi_read();   require !err;
-    (* ret = ret << 0 *)
-    unpack! addr, err = spi_read();  require !err;
+    unpack! ret, err = spi_xchg(constr:(Ox"0b"));        require !err; (* FASTREAD *)
+    unpack! ret, err = spi_xchg(addr >> constr:(8));     require !err;
+    unpack! ret, err = spi_xchg(addr & constr:(Ox"ff")); require !err;
+    unpack! ret, err = spi_xchg(err);                    require !err; (* dummy *)
+
+    unpack! ret, err = spi_xchg(err);                    require !err; (* read *)
+    unpack! addr, err = spi_xchg(err);                   require !err; (* read *)
     ret = (ret | (addr << constr:(8)));
-    unpack! addr, err = spi_read();  require !err;
+    unpack! addr, err = spi_xchg(err);                   require !err; (* read *)
     ret = (ret | (addr << constr:(16)));
-    unpack! addr, err = spi_read();  require !err;
+    unpack! addr, err = spi_xchg(err);                   require !err; (* read *)
     ret = (ret | (addr << constr:(24)));
 
     io! addr = MMIOREAD(SPI_CSMODE_ADDR);
@@ -51,8 +42,177 @@ Definition lan9250_readword : function :=
     output! MMIOWRITE(SPI_CSMODE_ADDR, addr)
   ))).
 
-Instance spec_of_lan9250_readword : ProgramLogic.spec_of "lan9250_readword" :=
-  fun functions => forall t m addr,
-    (Ox"0" <= Word.Interface.word.unsigned addr < Ox"400") ->
-    WeakestPrecondition.call functions "lan9250_readword" t m [addr] (fun T M RETS =>
-      M = m /\ exists v, RETS = [v]).
+Require Import bedrock2.ProgramLogic.
+Require Import bedrock2.FE310CSemantics.
+Require Import coqutil.Word.Interface.
+Require Import Coq.Lists.List. Import ListNotations.
+Require Import bedrock2.TracePredicate. Import TracePredicateNotations.
+Require bedrock2.Examples.lightbulb_spec.
+
+Import coqutil.Map.Interface.
+
+Instance spec_of_lan9250_readword : ProgramLogic.spec_of "lan9250_readword" := fun functions => forall t m a,
+  (Ox"0" <= Word.Interface.word.unsigned a < Ox"400") ->
+  WeakestPrecondition.call functions "lan9250_readword" t m [a] (fun T M RETS =>
+    M = m /\
+    exists ret err, RETS = [ret; err] /\
+    exists iol, T = iol ++ t /\
+    exists ioh, mmio_trace_abstraction_relation ioh iol /\ Logic.or
+      (word.unsigned err <> 0 /\ (any +++ lightbulb_spec.spi_timeout _) ioh)
+      (word.unsigned err = 0 /\ lightbulb_spec.lan9250_fastread4 _ _ a ret ioh)).
+
+From coqutil Require Import letexists.
+Local Ltac split_if :=
+  lazymatch goal with
+    |- WeakestPrecondition.cmd _ ?c _ _ _ ?post =>
+    let c := eval hnf in c in
+        lazymatch c with
+        | cmd.cond _ _ _ => letexists; split; [solve[repeat straightline]|split]
+        end
+  end.
+
+Lemma TracePredicate__any_app_more : forall {T} P (x y : list T), (any +++ P) x -> (any +++ P) (x ++ y).
+Proof.
+  intros.
+  cbv [any] in *.
+  destruct H as (?&?&?&?&?); subst.
+  rewrite <-app_assoc.
+  eapply concat_app; eauto.
+Qed.
+
+From coqutil Require Import Z.div_mod_to_equations.
+Lemma lan9250_readword_ok : program_logic_goal_for_function! lan9250_readword.
+Proof.
+  Time repeat straightline.
+
+  repeat match goal with
+    | H :  _ /\ _ \/ ?Y /\ _, G : not ?X |- _ =>
+        constr_eq X Y; let Z := fresh in destruct H as [|[Z ?]]; [|case (G Z)]
+    | H :  not ?Y /\ _ \/ _ /\ _, G : ?X |- _ =>
+        constr_eq X Y; let Z := fresh in destruct H as [[Z ?]|]; [case (Z G)|]
+    | _ => progress cbv [MMIOREAD MMIOWRITE]
+    | _ => progress cbv [SPI_CSMODE_ADDR]
+    | |- _ /\ _ => split
+    | |- context G[string_dec ?x ?x] =>
+        let e := eval cbv in (string_dec x x) in
+        let goal := context G [e] in
+        change goal
+    | |- context G[string_dec ?x ?y] =>
+        unshelve erewrite (_ : string_dec x y = right _); [ | exact eq_refl | ]
+    | _ => straightline_cleanup
+    | |- WeakestPrecondition.cmd _ (cmd.interact _ _ _) _ _ _ _ => eapply WeakestPreconditionProperties.interact_nomem
+    | |- Semantics.ext_spec _ _ _ _ _ => progress cbn [parameters Semantics.ext_spec]
+    | |- Ox _ <= word.unsigned (word.of_Z ?x) < Ox _ \/ _ => left; clear; cbv; clear; intuition congruence
+    | |- _ \/ Ox _ <= word.unsigned (word.of_Z ?x) < Ox _ => right; clear; cbv; clear; intuition congruence
+    | H: ?x = 0 |-  _ => rewrite H
+    | |- ?F ?a ?b ?c =>
+        match F with WeakestPrecondition.get => idtac end;
+        let f := (eval cbv beta delta [WeakestPrecondition.get] in F) in
+        change (f a b c); cbv beta
+    | _ => straightline
+    | _ => straightline_call
+    | _ => split_if
+  end.
+  all: try (eexists _, _; split; trivial).
+  all: try (exact eq_refl).
+  all: auto.
+
+  all : try (
+    repeat match goal with x := _ ++ _ |- _ => subst x end;
+    eexists; split;
+    [ repeat match goal with
+      |- context G [cons ?a ?b] =>
+        assert_fails (idtac; match b with nil => idtac end);
+        let goal := context G [(app (cons a nil) b)] in
+        change goal
+      end;
+    rewrite !app_assoc;
+    repeat eapply (fun A => f_equal2 (@List.app A)); eauto |]).
+
+  all : try (
+    eexists; split; [
+    repeat (eassumption || eapply Forall2_app || eapply Forall2_nil || eapply Forall2_cons) |]).
+  all : try ((left + right); eexists _, _; split; exact eq_refl).
+
+
+  all : try (left; split; [eassumption|]).
+  all : repeat rewrite <-app_assoc.
+
+  all : eauto using TracePredicate__any_app_more.
+
+  { rewrite Properties.word.unsigned_sru_nowrap by exact eq_refl.
+    1:change (word.unsigned (word.of_Z 8)) with 8.
+    rewrite Z.shiftr_div_pow2 by Omega.omega.
+    clear -H8.
+    change (Ox "400") with (4*256) in *.
+    Z.div_mod_to_equations. Lia.lia. }
+  { rewrite Properties.word.unsigned_and_nowrap.
+    change (word.unsigned (word.of_Z 255)) with (Z.ones 8).
+    rewrite Z.land_ones by Omega.omega.
+    Z.div_mod_to_equations. Lia.lia. }
+
+  right.
+  eexists; eauto.
+  eexists _, _,  _, _, _, _.
+
+  cbv [
+  lightbulb_spec.lan9250_fastread4
+  lightbulb_spec.spi_begin
+  lightbulb_spec.spi_xchg_mute
+  lightbulb_spec.spi_xchg_dummy
+  lightbulb_spec.spi_xchg_deaf
+  lightbulb_spec.spi_end
+  one
+  existsl
+  ].
+
+  cbv [concat].
+  repeat match goal with
+    | |- _ /\ _ => eexists
+    | |- exists _, _ => eexists
+    | |- ?e = _ => is_evar e; exact eq_refl
+    | |- _ = ?e => is_evar e; exact eq_refl
+  end.
+
+  1 : rewrite <-app_assoc.
+  1 : exact eq_refl.
+  all : try eassumption.
+  1,2:
+    repeat match goal with
+    | _ => rewrite word.of_Z_unsigned
+    | _ => rewrite word.unsigned_of_Z
+    | _ => cbv [word.wrap]; rewrite Z.mod_small
+    | _ => solve [trivial]
+    end.
+  { rewrite Properties.word.unsigned_sru_nowrap by exact eq_refl.
+    1:change (word.unsigned (word.of_Z 8)) with 8.
+    rewrite Z.shiftr_div_pow2 by Omega.omega.
+    revert dependent a; clear; intros.
+    change (Ox "400") with (4*256) in *. change (Ox "0") with 0 in *.
+    Z.div_mod_to_equations. Lia.lia. }
+  { rewrite Properties.word.unsigned_and_nowrap.
+    change (word.unsigned (word.of_Z 255)) with (Z.ones 8).
+    rewrite Z.land_ones by Omega.omega.
+    Z.div_mod_to_equations. Lia.lia. }
+  repeat match goal with x := _ |- _ => subst x end.
+  cbv [LittleEndian.combine PrimitivePair.pair._1 PrimitivePair.pair._2].
+  repeat rewrite ?Properties.word.unsigned_or_nowrap, <-?Z.lor_assoc by exact eq_refl.
+  change (Z.shiftl 0 8) with 0 in *; rewrite Z.lor_0_r.
+  rewrite !Z.shiftl_lor, !Z.shiftl_shiftl in * by Lia.lia.
+  repeat f_equal.
+
+  (* little-endian word conversion, automatable (bitwise Z and word) *)
+  all : try rewrite word.unsigned_slu by exact eq_refl.
+  all : match goal with |- context[word.unsigned (width:=?w) ?x] => is_var x; replace (word.unsigned (width:=w) x) with (word.wrap (width:=w) (word.unsigned (width:=w) x)) by eapply Properties.word.wrap_unsigned; set (word.unsigned (width:=w) x) as X; clearbody X end.
+  all : try erewrite ?word.unsigned_of_Z.
+  all : cbv [word.wrap].
+  all : change Semantics.width with 32.
+  all : repeat match goal with |- context G [?a mod ?b] => let goal := context G [a] in change goal end.
+  all : change (8+8) with 16.
+  all : change (8+16) with 24.
+  all : clear.
+  all : rewrite ?Z.shiftl_mul_pow2 by Lia.lia.
+  all : try (Z.div_mod_to_equations; Lia.lia).
+
+  Unshelve. all: intros; exact True.
+Qed.
