bedrock2/src/Examples/SPI.v
@@ -11,11 +11,13 @@ Local Coercion name_of_func (f : function) := fst f.
 Local Notation MMIOWRITE := "MMIOWRITE".
 Local Notation MMIOREAD := "MMIOREAD".
 
+Require bedrock2.Examples.lightbulb_spec.
+Local Notation patience := lightbulb_spec.patience.
+
 Definition spi_write : function :=
   let b : varname := "b" in
   let busy : varname := "busy" in
   let i : varname := "i" in
-  let patience := -1 in
   let SPI_WRITE_ADDR := Ox"10024048" in
   ("spi_write", ((b::nil), (busy::nil), bedrock_func_body:(
     busy = (constr:(-1));
@@ -35,11 +37,10 @@ Definition spi_read : function :=
   let b : varname := "b" in
   let busy : varname := "busy" in
   let i : varname := "i" in
-  let patience := -1 in
-  let SPI_READ_ADDR := Ox"0x1002404c" in
+  let SPI_READ_ADDR := Ox"1002404c" in
   ("spi_read", (nil, (b::busy::nil), bedrock_func_body:(
     busy = (constr:(-1));
-    b = (busy);
+    b = (constr:(Ox"5a"));
     i = (patience); while (i) { i = (i - constr:(1));
       io! busy = MMIOREAD(SPI_READ_ADDR);
       if !(busy >> constr:(31)) {
@@ -56,7 +57,7 @@ Definition spi_xchg : function :=
   ("spi_xchg", (b::nil, b::busy::nil, bedrock_func_body:(
     unpack! busy = spi_write(b);
     require !busy;
-    unpack! b, busy = spi_read(b)
+    unpack! b, busy = spi_read()
   ))).
 
 Require Import bedrock2.ProgramLogic.
@@ -64,9 +65,9 @@ Require Import bedrock2.FE310CSemantics.
 Require Import coqutil.Word.Interface.
 Require Import Coq.Lists.List. Import ListNotations.
 Require Import bedrock2.TracePredicate. Import TracePredicateNotations.
-Require bedrock2.Examples.lightbulb_spec.
 
 Import coqutil.Map.Interface.
+Import ReversedListNotations.
 
 Definition mmio_event_abstraction_relation
   (h : lightbulb_spec.OP Semantics.word)
@@ -76,25 +77,36 @@ Definition mmio_event_abstraction_relation
     (exists a v, h = lightbulb_spec.ld _ a v /\ l = (map.empty, "MMIOREAD", [a], (map.empty, [v]))).
 Definition mmio_trace_abstraction_relation := List.Forall2 mmio_event_abstraction_relation.
 
-Import ReversedListNotations.
 Instance spec_of_spi_write : spec_of "spi_write" := fun functions => forall t m b,
   word.unsigned b < 2 ^ 8 ->
   WeakestPrecondition.call functions "spi_write" t m [b] (fun T M RETS =>
-    M = m /\ exists iol, T = t ;++ iol /\ exists ioh, mmio_trace_abstraction_relation ioh iol /\ Logic.or
-      ((exists err, RETS = [err] /\ word.unsigned (word.sru err (word.of_Z 31)) <> 0))
-      (RETS = [word.of_Z 0] /\ lightbulb_spec.spi_write Semantics.byte Semantics.word (word.of_Z (word.unsigned b)) ioh)).
+    M = m /\ exists iol, T = t ;++ iol /\ exists ioh, mmio_trace_abstraction_relation ioh iol /\ exists err, RETS = [err] /\ Logic.or
+      (((word.unsigned err <> 0) /\ lightbulb_spec.spi_write_full _ ^* ioh /\ Z.of_nat (length ioh) = patience))
+      (word.unsigned err = 0 /\ lightbulb_spec.spi_write Semantics.byte Semantics.word (word.of_Z (word.unsigned b)) ioh)).
+
+Instance spec_of_spi_read : spec_of "spi_read" := fun functions => forall t m,
+  WeakestPrecondition.call functions "spi_read" t m [] (fun T M RETS =>
+    M = m /\ exists iol, T = t ;++ iol /\ exists ioh, mmio_trace_abstraction_relation ioh iol /\ exists (b:Semantics.byte) (err : Semantics.word), RETS = [word.of_Z (word.unsigned b); err] /\ Logic.or
+      (word.unsigned err <> 0 /\ lightbulb_spec.spi_read_empty _ ^* ioh /\ Z.of_nat (length ioh) = patience)
+      (word.unsigned err = 0 /\ lightbulb_spec.spi_read Semantics.byte Semantics.word b ioh)).
+
+Lemma nonzero_because_high_bit_set x (H : word.unsigned (word.sru x (word.of_Z 31)) <> 0)
+  : word.unsigned x <> 0.
+Proof.
+  rewrite Properties.word.unsigned_sru_nowrap in H by exact eq_refl.
+  intro HX.
+  rewrite HX in H.
+  exact (H eq_refl).
+Qed.
 
 Import coqutil.Tactics.letexists.
 Import TailRecursion.
-Lemma spi_write_ok : Semantics.parameters_ok parameters -> program_logic_goal_for_function! spi_write.
+Lemma spi_write_ok : program_logic_goal_for_function! spi_write.
 Proof.
-  intros p_ok.
   repeat straightline.
   rename H into Hb.
-  show_program.
 
   (* WHY do theese parentheses matter? *)
-  Fail refine (atleastonce ["b"; "busy"; "i"] (fun v t m b busy i => True) _ _ _ _ _ _ _).
   refine ((atleastonce ["b"; "busy"; "i"] (fun v T M B BUSY I =>
      b = B /\
      v = word.unsigned I /\
@@ -102,8 +114,9 @@ Proof.
      M = m /\
      exists tl, T = tl++t /\
      exists th, mmio_trace_abstraction_relation th tl /\
-     lightbulb_spec.spi_write_full _ ^* th))
-          _ _ _ _ _ _ _);
+     lightbulb_spec.spi_write_full _ ^* th /\
+     Z.of_nat (length th) + word.unsigned I = patience
+     )) _ _ _ _ _ _ _);
     cbn [reconstruct map.putmany_of_list HList.tuple.to_list
          HList.hlist.foralls HList.tuple.foralls
          HList.hlist.existss HList.tuple.existss
@@ -121,7 +134,11 @@ Proof.
     split; trivial.
     eexists; split.
     { rewrite app_nil_l; trivial. }
-    eexists; split; constructor. }
+    eexists; split.
+    { constructor. }
+    split.
+    { constructor. }
+    exact eq_refl. }
   repeat straightline.
   eapply WeakestPreconditionProperties.interact_nomem; repeat straightline.
   split.
@@ -139,12 +156,19 @@ Proof.
       { refine (List.Forall2_app _ _); try eassumption.
         econstructor; [|constructor].
         right; eexists _, _; repeat split. }
-      eapply kleene_app; eauto.
-      refine (kleene_step _ _ nil _ (kleene_empty _)).
-      repeat econstructor.
-      repeat match goal with x:=_|-_=>subst x end.
-      rewrite Properties.word.unsigned_sru_nowrap in H by exact eq_refl; eapply H. }
-    { split; try eapply Properties.word.decrement_nonzero_lt;
+      split.
+      { eapply kleene_app; eauto.
+        refine (kleene_step _ _ nil _ (kleene_empty _)).
+        repeat econstructor.
+        repeat match goal with x:=_|-_=>subst x end.
+        rewrite Properties.word.unsigned_sru_nowrap in H by exact eq_refl; eapply H. }
+      { rewrite app_length, Znat.Nat2Z.inj_add; cbn [app Datatypes.length]; subst i.
+        unshelve erewrite (_ : patience = _); [|symmetry; eassumption|].
+        rewrite word.unsigned_sub; cbv [word.wrap]; rewrite Z.mod_small; rewrite Properties.word.unsigned_of_Z_1.
+        2: { pose proof Properties.word.unsigned_range x1.
+             change Semantics.width with 32 in *. Lia.lia. }
+        ring. } }
+      { split; try eapply Properties.word.decrement_nonzero_lt;
         try eapply Properties.word.unsigned_range; eauto. } }
   { letexists; split; [solve[repeat straightline]|split]; repeat straightline; try contradiction.
     split; eauto.
@@ -155,7 +179,21 @@ Proof.
     { eapply Forall2_app; eauto.
       constructor; [|constructor].
       right; eauto. }
-    { left; repeat split; eauto. } }
+    eexists. split; trivial.
+    { left; repeat split; eauto using nonzero_because_high_bit_set.
+      { (* copied from above -- trace element for "fifo full" *)
+        eapply kleene_app; eauto.
+        refine (kleene_step _ _ nil _ (kleene_empty _)).
+        repeat econstructor.
+        repeat match goal with x:=_|-_=>subst x end.
+        rewrite Properties.word.unsigned_sru_nowrap in H by exact eq_refl; eapply H. }
+      { rewrite app_length, Znat.Nat2Z.inj_add; cbn [app Datatypes.length]; subst i.
+        unshelve erewrite (_ : patience = _); [|symmetry; eassumption|].
+        change 0 with (word.unsigned (word.of_Z 0)) in H0.
+        eapply Properties.word.unsigned_inj in H0.
+        assert (HA: word.add (word.sub x1 (word.of_Z 1)) (word.of_Z 1) = word.of_Z 1). {
+          match goal with H : _ |- _ => rewrite H; ring end. }
+        ring_simplify in HA; subst. ring_simplify; reflexivity. } } }
   { do 3 letexists; repeat straightline.
     subst i.
     rewrite Properties.word.unsigned_xor_nowrap in *; rewrite Z.lxor_nilpotent in *; contradiction. }
@@ -176,11 +214,11 @@ Proof.
       { left. eexists _, _; repeat split. }
       { right; [|constructor].
         right; eexists _, _; repeat split. } } }
+  eexists; split; trivial.
   right.
   subst busy.
   split.
-  { f_equal. eapply Properties.word.unsigned_inj.
-    rewrite Properties.word.unsigned_xor_nowrap; rewrite Z.lxor_nilpotent; reflexivity. }
+  { f_equal. rewrite Properties.word.unsigned_xor_nowrap; rewrite Z.lxor_nilpotent; reflexivity. }
   cbv [lightbulb_spec.spi_write].
   eexists _, _; split; eauto; []; split; eauto.
   eexists (cons _ nil), (cons _ nil); split; cbn [app]; eauto.
@@ -191,10 +229,249 @@ Proof.
     repeat f_equal.
     eapply Properties.word.unsigned_inj.
     clear -Hb.
-    pose proof Properties.word.unsigned_range b.
+    pose proof Properties.word.unsigned_range x.
     change (Semantics.width) with 32 in *.
     do 2 (rewrite word.unsigned_of_Z; cbv [word.wrap]; rewrite Z.mod_small); Lia.lia. }
   
   Unshelve.
   all : intros; exact True.
+Qed.
+
+Local Ltac split_if :=
+  lazymatch goal with
+    |- WeakestPrecondition.cmd _ ?c _ _ _ ?post =>
+    let c := eval hnf in c in
+        lazymatch c with
+        | cmd.cond _ _ _ => letexists; split; [solve[repeat straightline]|split]
+        end
+  end.
+
+Lemma spi_read_ok : program_logic_goal_for_function! spi_read.
+  repeat straightline.
+  refine ((atleastonce ["b"; "busy"; "i"] (fun v T M B BUSY I =>
+     v = word.unsigned I /\
+     word.unsigned I <> 0 /\
+     M = m /\
+     B = word.of_Z (word.unsigned (width:=8) (word.of_Z (word.unsigned B))) /\
+     exists tl, T = tl++t /\
+     exists th, mmio_trace_abstraction_relation th tl /\
+     lightbulb_spec.spi_read_empty _ ^* th /\
+     Z.of_nat (length th) + word.unsigned I = patience
+          ))
+          _ _ _ _ _ _ _);
+    cbn [reconstruct map.putmany_of_list HList.tuple.to_list
+         HList.hlist.foralls HList.tuple.foralls
+         HList.hlist.existss HList.tuple.existss
+         HList.hlist.apply  HList.tuple.apply
+         HList.hlist
+         List.repeat Datatypes.length
+         HList.polymorphic_list.repeat HList.polymorphic_list.length
+         PrimitivePair.pair._1 PrimitivePair.pair._2] in *; repeat straightline.
+  { exact (Z.lt_wf 0). }
+  { inversion H. }
+  { split; trivial.
+    split; [inversion 1|].
+    split; trivial.
+    split; trivial.
+    eexists nil; split; trivial.
+    eexists nil; split; try split; solve [constructor]. }
+  { eapply WeakestPreconditionProperties.interact_nomem; repeat straightline.
+    split; change (Naive.word 32) with Semantics.word.
+    { cbv; clear; intuition congruence. }
+    repeat ((split; trivial; []) || straightline || split_if).
+    { repeat letexists.
+      split.
+      { repeat straightline. }
+      repeat ((split; trivial; []) || straightline || split_if).
+      letexists. split; split.
+      { subst v'; exact eq_refl. }
+      { split; trivial.
+        split; trivial.
+        split; trivial.
+        eexists (x2 ;++ cons _ nil); split; cbn [app]; eauto.
+        eexists. split.
+        { econstructor; try eassumption; right; eauto. }
+        split.
+        { 
+          refine (kleene_app _ (cons _ nil) _ x3 _); eauto.
+          refine (kleene_step _ (cons _ nil) nil _ (kleene_empty _)).
+          eexists; split.
+          { exact eq_refl. }
+          { subst v1.
+            rewrite Properties.word.unsigned_sru_nowrap in H by exact eq_refl; exact H. } }
+        { cbn [Datatypes.length]; subst i.
+          unshelve erewrite (_ : patience = _); [|symmetry; eassumption|].
+          rewrite word.unsigned_sub; cbv [word.wrap]; rewrite Z.mod_small; rewrite Properties.word.unsigned_of_Z_1.
+          2: { pose proof Properties.word.unsigned_range x1.
+               change Semantics.width with 32 in *. Lia.lia. }
+          Lia.lia. } }
+        { eapply Properties.word.unsigned_range. }
+        { eapply Properties.word.decrement_nonzero_lt; eassumption. }}
+    { letexists; split; repeat straightline.
+      split; trivial.
+      eexists (x2 ;++ cons _ nil); split; cbn [app]; eauto.
+      eexists. split.
+      { econstructor; try eassumption; right; eauto. }
+      eexists (word.of_Z (word.unsigned x)), _; split.
+      { f_equal; congruence. }
+      left; repeat split; eauto using nonzero_because_high_bit_set.
+      { refine (kleene_app _ (cons _ nil) _ x3 _); eauto.
+        refine (kleene_step _ (cons _ nil) nil _ (kleene_empty _)).
+        eexists; split.
+        { exact eq_refl. }
+        { subst v1.
+          rewrite Properties.word.unsigned_sru_nowrap in H by exact eq_refl; exact H. } }
+      { cbn [Datatypes.length]; subst i.
+        unshelve erewrite (_ : patience = _); [|symmetry; eassumption|].
+        change 0 with (word.unsigned (word.of_Z 0)) in H1.
+        eapply Properties.word.unsigned_inj in H1.
+        assert (HA: word.add (word.sub x1 (word.of_Z 1)) (word.of_Z 1) = word.of_Z 1). {
+          match goal with H : _ |- _ => rewrite H; ring end. }
+        ring_simplify in HA; subst. rewrite Properties.word.unsigned_of_Z_1; Lia.lia. } }
+    { repeat straightline.
+      repeat letexists; split.
+      { repeat straightline. }
+      repeat letexists; split.
+      1: split.
+      { repeat straightline. }
+      2: {
+        subst v'.
+        subst v.
+        subst i.
+        rewrite Properties.word.unsigned_xor_nowrap, Z.lxor_nilpotent.
+        pose proof Properties.word.unsigned_range x1. Lia.lia. }
+      repeat straightline.
+      repeat (split; trivial; []).
+      split.
+      { subst b.
+        (* automatable: multi-word bitwise *)
+        change (255) with (Z.ones 8).
+        pose proof Properties.word.unsigned_range v0.
+        eapply Properties.word.unsigned_inj;
+          repeat (
+              cbv [word.wrap];
+              rewrite ?word.unsigned_of_Z, ?Properties.word.unsigned_and_nowrap, ?Z.land_ones, ?Z.mod_mod, ?Z.mod_small by Lia.lia;
+              change (Z.ones 8 mod 2 ^ Semantics.width) with (Z.ones 8)).
+        symmetry; eapply Z.mod_small.
+        pose proof Z.mod_pos_bound (word.unsigned v0) (2^8) eq_refl.
+        change Semantics.width with 32.
+        Lia.lia. }
+      { (* copy-paste from above, trace manipulation *)
+        eexists (x2 ;++ cons _ nil); split; cbn [app]; eauto.
+        eexists. split.
+        { econstructor; try eassumption; right; eauto. }
+        subst i.
+        rewrite Properties.word.unsigned_xor_nowrap, Z.lxor_nilpotent in H1; contradiction. } }
+    { eexists _; split.
+      { repeat straightline. }
+      split; trivial.
+      (* copy-paste from above, trace manipulation *)
+      eexists (x2 ;++ cons _ nil); split; cbn [app]; eauto.
+      eexists. split.
+      { econstructor; try eassumption; right; eauto. }
+      eexists (word.of_Z (word.unsigned b)), _; split.
+      { subst b; f_equal.
+        (* automatable: multi-word bitwise *)
+        change (255) with (Z.ones 8).
+        pose proof Properties.word.unsigned_range v0.
+        eapply Properties.word.unsigned_inj;
+          repeat (
+              cbv [word.wrap];
+              rewrite ?word.unsigned_of_Z, ?Properties.word.unsigned_and_nowrap, ?Z.land_ones, ?Z.mod_mod, ?Z.mod_small by Lia.lia;
+              change (Z.ones 8 mod 2 ^ Semantics.width) with (Z.ones 8)).
+        symmetry; eapply Z.mod_small.
+        pose proof Z.mod_pos_bound (word.unsigned v0) (2^8) eq_refl.
+        change Semantics.width with 32.
+        Lia.lia. }
+      { right; split.
+        { subst busy. rewrite Properties.word.unsigned_xor_nowrap, Z.lxor_nilpotent; exact eq_refl. }
+        eexists x3, (cons _ nil); split; cbn [app]; eauto.
+        split; eauto.
+        eexists; split; cbv [one]; trivial.
+        split.
+        { subst v1. rewrite Properties.word.unsigned_sru_nowrap in H by exact eq_refl; exact H. }
+        subst b.
+        (* automatable: multi-word bitwise *)
+        change (255) with (Z.ones 8).
+        pose proof Properties.word.unsigned_range v0.
+        eapply Properties.word.unsigned_inj;
+          repeat (
+              cbv [word.wrap];
+              rewrite ?word.unsigned_of_Z, ?Properties.word.unsigned_and_nowrap, ?Z.land_ones, ?Z.mod_mod, ?Z.mod_small by Lia.lia;
+              change (Z.ones 8 mod 2 ^ Semantics.width) with (Z.ones 8)).
+        trivial. } } }
+  Unshelve.
+  intros. exact True. (* WHY do we have this shelved predicate here? *)
+Qed.
+
+Instance spec_of_spi_xchg : spec_of "spi_xchg" := fun functions => forall t m b_out,
+  word.unsigned b_out < 2 ^ 8 ->
+  WeakestPrecondition.call functions "spi_xchg" t m [b_out] (fun T M RETS =>
+    M = m /\ exists iol, T = t ;++ iol /\ exists ioh, mmio_trace_abstraction_relation ioh iol /\ exists (b_in:Semantics.byte) (err : Semantics.word), RETS = [word.of_Z (word.unsigned b_in); err] /\ Logic.or
+      (word.unsigned err <> 0 /\ (any +++ lightbulb_spec.spi_timeout _) ioh)
+      (word.unsigned err = 0 /\ lightbulb_spec.spi_xchg Semantics.byte Semantics.word (word.of_Z (word.unsigned b_out)) b_in ioh)).
+
+Lemma spi_xchg_ok : program_logic_goal_for_function! spi_xchg.
+Proof.
+  repeat (
+  match goal with
+  | |- ?F ?a ?b ?c =>
+      match F with WeakestPrecondition.get => idtac end;
+      let f := (eval cbv beta delta [WeakestPrecondition.get] in F) in
+      change (f a b c); cbv beta
+    | H :  _ /\ _ \/ ?Y /\ _, G : not ?X |- _ =>
+        constr_eq X Y; let Z := fresh in destruct H as [|[Z ?]]; [|case (G Z)]
+    | H :  not ?Y /\ _ \/ _ /\ _, G : ?X |- _ =>
+        constr_eq X Y; let Z := fresh in destruct H as [[Z ?]|]; [case (Z G)|]
+  end ||
+
+  straightline || straightline_call || split_if || refine (conj _ _) || eauto).
+
+{ eexists. split.
+  { exact eq_refl. }
+  eexists. split.
+  { eauto. }
+  eexists. eexists. split.
+  { repeat f_equal. 
+    instantiate (1 := (word.of_Z (word.unsigned b_out) : Semantics.byte)).
+    (* automatable: multi-word bitwise *)
+    change (255) with (Z.ones 8).
+    pose proof Properties.word.unsigned_range b_out.
+    eapply Properties.word.unsigned_inj;
+    repeat (
+    cbv [word.wrap];
+    rewrite ?word.unsigned_of_Z, ?Properties.word.unsigned_and_nowrap, ?Z.land_ones, ?Z.mod_mod, ?Z.mod_small by Lia.lia;
+    change (Z.ones 8 mod 2 ^ Semantics.width) with (Z.ones 8)).
+    rewrite Z.mod_small; rewrite Z.mod_small; trivial; Lia.lia. }
+    left; split; eauto.
+    eexists nil, x0; repeat split; cbv [any choice lightbulb_spec.spi_timeout]; eauto.
+    rewrite app_nil_r; trivial. }
+
+    { destruct H10; intuition eauto.
+      { eexists. split.
+        { subst a0. subst a.
+          rewrite List.app_assoc; trivial. }
+          eexists. split.
+          { eapply Forall2_app; eauto. }
+          eexists _, _; split.
+          { subst v; trivial. }
+          left; split; eauto.
+          eapply concat_app; cbv [any choice lightbulb_spec.spi_timeout]; eauto. }
+          eexists.
+          subst a0.
+          subst a.
+          split.
+          { rewrite List.app_assoc; trivial. }
+          eexists.
+          split.
+          { eapply Forall2_app; eauto. }
+          eexists _, _; split.
+          { subst v. eauto. }
+          right. split; eauto.
+          cbv [lightbulb_spec.spi_xchg].
+
+assert (Trace__concat_app : forall T (P Q:list T->Prop) x y, P x -> Q y -> (P +++ Q) (y ++ x)). {
+  cbv [concat]; eauto. }
+
+  eauto using Trace__concat_app. }
 Qed.
