bedrock2/src/Examples/lightbulb.v
@@ -22,46 +22,31 @@ Lemma word__unsigned_of_Z_nowrap x : 0 <= x < 2 ^ width -> word.unsigned (word.o
 Proof.
   intros. rewrite word.unsigned_of_Z. unfold word.wrap. rewrite Z.mod_small; trivial.
 Qed.
-Ltac seplog_use_array_load1 H i :=
+Local Ltac seplog_use_array_load1 H i :=
   let iNat := eval cbv in (Z.to_nat i) in
   let H0 := fresh in pose proof H as H0;
   unshelve SeparationLogic.seprewrite_in @array_index_nat_inbounds H0;
     [exact iNat|exact (word.of_Z 0)|blia|];
   change ((word.unsigned (word.of_Z 1) * Z.of_nat iNat)%Z) with i in *.
-Ltac trans_ltu :=
-          match goal with
-          H : word.unsigned ?v <> 0 |- _ =>
-          let v := rdelta.rdelta v in
-          let __ := lazymatch v with if word.ltu _ _ then word.of_Z 1 else word.of_Z 0 => I end in
-          eapply Properties.word.if_nonzero in H; rewrite word.unsigned_ltu in H; eapply Z.ltb_lt in H end.
-Ltac straightline_if :=
+Local Ltac trans_ltu :=
+  match goal with
+  | H : word.unsigned ?v <> 0 |- _ =>
+      let v := rdelta.rdelta v in
+      let __ := lazymatch v with if word.ltu _ _ then word.of_Z 1 else word.of_Z 0 => I end in
+      eapply Properties.word.if_nonzero in H; rewrite word.unsigned_ltu in H; eapply Z.ltb_lt in H
+  | H : word.unsigned ?v = 0 |- _ =>
+      let v := rdelta.rdelta v in
+      let __ := lazymatch v with if word.ltu _ _ then word.of_Z 1 else word.of_Z 0 => I end in
+      eapply Word.Properties.word.if_zero in H; rewrite word.unsigned_ltu in H; eapply Z.ltb_nlt in H
+end.
+Local Ltac split_if :=
   lazymatch goal with
-  |- WeakestPrecondition.cmd _ ?c _ _ _ ?post =>
-        let c := eval hnf in c in
+    |- WeakestPrecondition.cmd _ ?c _ _ _ ?post =>
+    let c := eval hnf in c in
         lazymatch c with
-        | cmd.cond _ _ _ => letexists; split; [|split]
+        | cmd.cond _ _ _ => letexists; split; [solve[repeat straightline]|split]
         end
   end.
-Lemma interact_nomem call action binds arges t m l post
-  args (Hargs : dexprs m l arges args)
-  (Hext : ext_spec t map.empty binds args (fun mReceive (rets : list word) =>
-    mReceive = map.empty /\
-    exists l0 : locals, map.putmany_of_list action rets l = Some l0 /\
-    post ((map.empty, binds, args, (map.empty, rets)) :: t) m l0))
-  : WeakestPrecondition.cmd call (cmd.interact action binds arges) t m l post.
-Proof.
-  repeat straightline.
-  exists args; split; [exact Hargs|].
-  exists m.
-  exists map.empty.
-  split; [eapply Properties.map.split_empty_r; exact eq_refl|].
-  eapply ok; [|eapply Hext]; intros ? ? [? [? []]]; subst.
-  eexists; split; [eassumption|].
-  Print WeakestPrecondition.cmd_body.
-  eexists; split; [eapply Properties.map.split_empty_r; exact eq_refl|].
-  assumption.
-Qed.
-
 
 
 Definition main: cmd :=
@@ -78,26 +63,32 @@ Definition iot :=
     let bytesWritten : varname := "bytesWritten" in
     let recvEthernet : varname := "recvEthernet" in
     let lightbulb : varname := "lightbulb" in
-    let r : varname := "r" in
+    let err : varname := "err" in
 
-  ("iot", ((p_addr::nil), (r::nil), bedrock_func_body:(
-    unpack! bytesWritten = recvEthernet(p_addr);
-    require (bytesWritten ^ constr:(-1)) else { r = (constr:(-1)) };
-    unpack! r = lightbulb(p_addr, bytesWritten);
-
-    r = (constr:(0))
+  ("iot", ((p_addr::nil), (err::nil), bedrock_func_body:(
+    unpack! bytesWritten, err = recvEthernet(p_addr);
+    if !err { (* success, packet *)
+      unpack! err = lightbulb(p_addr, bytesWritten);
+      err = (constr:(0)) (* bad packet continue anyway *)
+    } else if !(err ^ constr:(1)) { (* success, no packet *)
+      err = (constr:(0))
+    }
   ))).
 
 Definition recvEthernet :=
     let buf : varname := "buf" in
     let num_bytes : varname := "num_bytes" in
     let i : varname := "i" in
+    let err : varname := "err" in
     let read : varname := "read" in
 
-    ("recvEthernet", ((buf::nil), (num_bytes::nil), bedrock_func_body:(
-        unpack! read = lan9250_readword(constr:(Ox"7C")); (* RX_FIFO_INF *)
-        require (read & constr:((2^8-1)*2^16)) else { num_bytes = (constr:(-1)) }; (* nonempty *)
-        unpack! read = lan9250_readword(constr:(Ox"40")); (* RX_STATUS_FIFO_PORT *)
+    ("recvEthernet", ((buf::nil), (num_bytes::err::nil), bedrock_func_body:(
+        num_bytes = (constr:(0));
+        unpack! read, err = lan9250_readword(constr:(Ox"7C")); (* RX_FIFO_INF *)
+        require !err else { err = (constr:(-1)) };
+        require (read & constr:((2^8-1)*2^16)) else { err = (constr:(1)) }; (* nonempty *)
+        unpack! read, err = lan9250_readword(constr:(Ox"40")); (* RX_STATUS_FIFO_PORT *)
+        require !err else { err = (constr:(-1)) };
 
         num_bytes = (read >> constr:(16) & constr:(2^14-1));
         (* round up to next word *)
@@ -105,12 +96,12 @@ Definition recvEthernet :=
         num_bytes = (num_bytes + num_bytes);
         num_bytes = (num_bytes + num_bytes);
 
-        require (num_bytes < constr:(1520 + 1)) else { num_bytes = (constr:(-1)) };
+        require (num_bytes < constr:(1520 + 1)) else { err = (constr:(2)) };
 
         i = (constr:(0)); while (i < num_bytes) {
-            unpack! read = lan9250_readword(constr:(0));
-            store4(buf + i, read);
-            i = (i + constr:(4))
+            unpack! read, err = lan9250_readword(constr:(0));
+            if err { err = (constr:(-1)); i = (num_bytes) }
+            else { store4(buf + i, read); i = (i + constr:(4)) }
         }
     ))).
 
@@ -142,11 +133,13 @@ Definition lightbulb :=
 
     r = (constr:(42));
     r = (packet + r);
-    command = (load1(r)); (* TODO: MMIOWRITE one bit only *)
+    command = (load1(r));
     command = (command&constr:(1));
 
+    (* pin output enable -- TODO do this in init
     io! mmio_val = MMIOREAD(constr:(Ox"10012008"));
     output! MMIOWRITE(constr:(Ox"10012008"), mmio_val | constr:(2^23));
+    *)
 
     r = (constr:(Ox"1001200c"));
     io! mmio_val = MMIOREAD(r);
@@ -156,85 +149,207 @@ Definition lightbulb :=
     r = (constr:(0))
   ))).
 
-Local Infix "*" := sep.
-Local Infix "*" := sep : type_scope.
+Import Datatypes List.
+Local Notation bytes := (array scalar8 (word.of_Z 1)).
+Local Infix "*" := (sep).
+Local Infix "*" := (sep) : type_scope.
 
-Instance spec_of_iot : spec_of "iot" := fun functions =>
-  forall p_addr buf R m t,
-    (array scalar8 (word.of_Z 1) p_addr buf * R) m ->
-    Z.of_nat (List.length buf) = 1520 ->
-    WeakestPrecondition.call functions "iot" t m [p_addr]
-      (fun t' m' rets => exists v, rets = [v]).
+Import TracePredicate. Import TracePredicateNotations.
+Import Word.Properties.
+Import lightbulb_spec.
 
 Instance spec_of_recvEthernet : spec_of "recvEthernet" := fun functions =>
   forall p_addr (buf:list byte) R m t,
     (array scalar8 (word.of_Z 1) p_addr buf * R) m ->
-    List.length buf = 1520%nat ->
-    (* comment on wormhole mentions < 0x400 for lan9250_readword. TODO check against manual *)
-    WeakestPrecondition.call functions "recvEthernet" t m [p_addr]
-      (fun t' m' rets =>
-       (* Success, we wrote 0+ bytes to the buffer *)
-       (
-         exists bytes_written:word, rets = [bytes_written]
-         /\
-         exists rx_packet', (array scalar8 (word.of_Z 1) p_addr rx_packet' *
-                             array scalar8 (word.of_Z 1) (word.add p_addr bytes_written)
-                                                         (List.skipn (Z.to_nat (word.unsigned bytes_written)) buf) *
-                             R) m'
-         /\
-         word.unsigned bytes_written <= Z.of_nat (List.length rx_packet')
-       )
-       \/
-       (* Fail, we return -1 and don't write anything *)
-       (rets = [word.of_Z (-1)] /\ m' = m)
+    length buf = 1520%nat ->
+    WeakestPrecondition.call functions "recvEthernet" t m [p_addr] (fun t' m' rets =>
+      exists bytes_written err, rets = [bytes_written; err] /\
+      exists iol, t' = iol ++ t /\
+      exists ioh, mmio_trace_abstraction_relation ioh iol /\ Logic.or
+        (word.unsigned err = 0 /\
+          exists recv buf, (bytes p_addr recv * bytes (word.add p_addr bytes_written) buf * R) m' /\ lan9250_recv _ _ recv ioh /\
+          word.unsigned bytes_written + Z.of_nat (length buf) = 1520%Z /\
+          Z.of_nat (length recv) = word.unsigned bytes_written)
+        (word.unsigned err <> 0 /\ exists buf, (array scalar8 (word.of_Z 1) p_addr buf * R) m' /\ length buf = 1520%nat /\ (
+           word.unsigned err = 1 /\ lan9250_recv_no_packet _ _ ioh \/
+           word.unsigned err = 2 /\ lan9250_recv_packet_too_long _ _ ioh \/
+           word.unsigned err = 2^32-1 /\ TracePredicate.concat TracePredicate.any (spi_timeout word) ioh
+          ))
       ).
+
+Definition lightbulb_packet_rep cmd (buf : list byte) :=
+  let idx i buf := word.of_Z (word.unsigned (List.hd (word.of_Z 0) (List.skipn i buf))) in
+  42 < Z.of_nat (length buf) /\
+  1535 < word.unsigned ((word.or (word.slu (idx 12%nat buf) (word.of_Z 8)) (idx 13%nat buf))) /\
+  idx 23%nat buf = word.of_Z (Ox"11") /\
+  cmd = Z.testbit (word.unsigned (List.hd (word.of_Z 0) (List.skipn 42 buf))) 0.
 
 Instance spec_of_lightbulb : spec_of "lightbulb" := fun functions =>
   forall p_addr (buf:list byte) (len:word) R m t,
     (array scalar8 (word.of_Z 1) p_addr buf * R) m ->
-    word.unsigned len <= Z.of_nat (List.length buf) ->
+    word.unsigned len = Z.of_nat (List.length buf) ->
     WeakestPrecondition.call functions "lightbulb" t m [p_addr; len]
-      (fun t' m' rets => exists v, rets = [v] /\ m' = m).
+      (fun t' m' rets => exists v, rets = [v] /\ m' = m /\ 
+      exists iol, t' = iol ++ t /\
+      exists ioh, mmio_trace_abstraction_relation ioh iol /\ Logic.or
+        (exists cmd, lightbulb_packet_rep cmd buf /\ gpio_set _ 23 cmd ioh /\ word.unsigned v = 0)
+        (not (exists cmd, lightbulb_packet_rep cmd buf) /\ ioh = nil /\ word.unsigned v <> 0)
+      ).
 
+Instance spec_of_iot : spec_of "iot" := fun functions =>
+  forall p_addr buf R m t,
+    (bytes p_addr buf * R) m ->
+    Z.of_nat (length buf) = 1520 ->
+    WeakestPrecondition.call functions "iot" t m [p_addr]
+      (fun t' m' rets => exists v, rets = [v] /\
+      exists iol, t' = iol ++ t /\
+      exists ioh, mmio_trace_abstraction_relation ioh iol /\ (
+        (exists packet cmd, (lan9250_recv _ _ packet +++ gpio_set _ 23 cmd) ioh /\ lightbulb_packet_rep cmd packet /\ word.unsigned v = 0) \/
+        (exists packet, (lan9250_recv _ _ packet) ioh /\ not (exists cmd, lightbulb_packet_rep cmd packet) /\ word.unsigned v = 0) \/
+        (lan9250_recv_no_packet _ _ ioh /\ word.unsigned v = 0) \/
+        (lan9250_recv_packet_too_long _ _ ioh /\ word.unsigned v <> 0) \/
+        ((TracePredicate.any +++ (spi_timeout word)) ioh /\ word.unsigned v <> 0)
+      )).
+
+Require Import bedrock2.AbsintWordToZ.
+Import WeakestPreconditionProperties.
+
+Lemma align_trace_cons {T} x xs cont t (H : xs = cont ++ t) : @cons T x xs = (cons x cont) ++ t.
+Proof. intros. cbn. congruence. Qed.
+Lemma align_trace_app {T} x xs cont t (H : xs = cont ++ t) : @app T x xs = (app x cont) ++ t.
+Proof. intros. cbn. subst. rewrite List.app_assoc; trivial. Qed.
 
 Lemma iot_ok : program_logic_goal_for_function! iot.
 Proof.
-  repeat (straightline || straightline_call || ecancel_assumption).
-  { blia. }
-  match goal with H : or _ _ |- _ => destruct H end;
-  repeat (straightline || straightline_call || straightline_if || ecancel_assumption || eauto).
-  match goal with H : _ |- _ => case (H eq_refl) end.
+  repeat (match goal with H : or _ _ |- _ => destruct H; intuition idtac end
+        || straightline || straightline_call || split_if || ecancel_assumption || eauto || blia).
+  all : eexists; split; [solve[eauto]|].
+  all : eexists; split.
+  all: repeat (eapply align_trace_cons || exact (eq_sym (List.app_nil_l _)) || eapply align_trace_app).
+  all : eexists; split.
+  all : repeat (eapply List.Forall2_cons || eapply List.Forall2_refl || eapply List.Forall2_app || eauto 15 using concat_app).
+
+  { subst v. rewrite word.unsigned_xor_nowrap, H10 in H4. case (H4 eq_refl). }
+  { subst v. rewrite word.unsigned_xor_nowrap, H9 in H4. inversion H4. }
+  { subst v. rewrite word.unsigned_xor_nowrap, H9 in H4. inversion H4. }
 Qed.
 
-Ltac prove_ext_spec :=
+Local Ltac prove_ext_spec :=
   lazymatch goal with
   | |- ext_spec _ _ _ _ _ => split; [cbv; clear; firstorder congruence|]; split; [trivial|]
   end.
+
+Local Ltac zify_unsigned :=
+  repeat match goal with
+  | |- context[word.unsigned ?e] => let H := unsigned.zify_expr e in rewrite H; pose proof H
+  | G : context[word.unsigned ?e] |- _ => let H := unsigned.zify_expr e in rewrite H in G; pose proof H
+  end;
+  repeat match goal with H:absint_eq ?x ?x |- _ => clear H end;
+  repeat match goal with H:?A |- _ => clear H; match goal with G:A |- _ => idtac end end.
+
+Lemma lightbulb_ok : program_logic_goal_for_function! lightbulb.
+Proof.
+  repeat (eauto || straightline || split_if || eapply interact_nomem || prove_ext_spec || trans_ltu).
+  all : subst r; try subst r0; change (word.unsigned (word.of_Z 42)) with 42 in *.
+
+  2: { eexists; split; [solve[eauto]|].
+    split; [solve[eauto]|].
+    eexists nil; split; eauto.
+    eexists nil; split; cbv [mmio_trace_abstraction_relation]; eauto using List.Forall2_refl.
+    right; repeat split; eauto. 
+    { intros (?&?&?). blia. }
+    intros HX; inversion HX. }
+
+  seplog_use_array_load1 H 12.
+  seplog_use_array_load1 H 13.
+  seplog_use_array_load1 H 23.
+  seplog_use_array_load1 H 42.
+  repeat (eauto || straightline || split_if || eapply interact_nomem || prove_ext_spec).
+
+  all : eexists; split; [solve[eauto]|].
+  all : split; [solve[eauto]|].
+  all : eexists; split.
+  all: repeat (eapply align_trace_cons || exact (eq_sym (List.app_nil_l _))).
+  all : eexists; split.
+
+  all : repeat (eapply List.Forall2_cons || eapply List.Forall2_refl).
+  all : 
+  try match goal with
+  |- mmio_event_abstraction_relation _ _ =>
+      (left+right); eexists _, _; split; exact eq_refl
+  end. 
+
+  all : repeat trans_ltu;
+  repeat match goal with
+  | H : word.unsigned ?v <> 0 |- _ =>
+      let v := rdelta.rdelta v in
+      let __ := lazymatch v with if word.eqb _ _ then word.of_Z 1 else word.of_Z 0 => I end in
+      eapply Properties.word.if_nonzero in H; eapply word.eqb_true in H
+  | H : word.unsigned ?v = 0 |- _ =>
+      let v := rdelta.rdelta v in
+      let __ := lazymatch v with if word.eqb _ _ then word.of_Z 1 else word.of_Z 0 => I end in
+      eapply Word.Properties.word.if_zero in H; eapply word.eqb_false in H
+  end;
+  repeat match goal with x := word.of_Z _ |- _ => subst x end.
+
+  1: {
+    left.
+    eexists; repeat split.
+    all : try eassumption.
+    1: blia.
+    cbv [gpio_set one existsl concat].
+    eexists _, ([_]), ([_]); repeat split; repeat f_equal.
+    subst command.
+    eapply word.unsigned_inj.
+    rewrite ?word.unsigned_and_nowrap.
+    change (word.unsigned (word.of_Z 1)) with (Z.ones 1).
+    rewrite Z.land_ones, Z.bit0_mod by blia.
+    rewrite !word.unsigned_of_Z.
+    cbv [word.wrap]; change width with 32 in *.
+    rewrite 2(Z.mod_small _ (2^32)); try exact eq_refl.
+    1: match goal with |- 0 <= word.unsigned ?x < _ => pose proof word.unsigned_range x end; blia.
+    1: clear; Z.div_mod_to_equations; blia. }
+
+  (* parse failures *)
+  all : right; repeat split; eauto; try solve[intros HX; inversion HX]; intros (?&?&?&?&?).
+  all : cbn in *; congruence.
+
+  Unshelve.
+  all : intros; exact True.
+Qed.
+
 
 Lemma recvEthernet_ok : program_logic_goal_for_function! recvEthernet.
 Proof.
   straightline.
   rename H into Hcall; clear H0 H1. rename H2 into H. rename H3 into H0.
-  repeat (straightline || straightline_if || straightline_call || eauto 99 || prove_ext_spec).
-  1,2: cbv - [Z.le Z.lt]; clear; blia.
-  refine (TailRecursion.tailrec
-    (* types of ghost variables *) (HList.polymorphic_list.cons (list byte) (HList.polymorphic_list.cons (mem -> Prop) HList.polymorphic_list.nil))
-    (* program variables *) ["buf";"num_bytes";"i";"read"]
-    (fun v scratch R t m buf num_bytes_loop i read =>
-      PrimitivePair.pair.mk (v = word.unsigned i /\
-      (array scalar8 (word.of_Z 1) (word.add buf i) scratch * R) m /\
-      Z.of_nat (List.length scratch) = word.unsigned (word.sub num_bytes i) /\
+  repeat (straightline || split_if || straightline_call || eauto 99 || prove_ext_spec).
+  1, 3: cbv - [Z.le Z.lt]; clear; blia.
 
+  3: {
+
+  refine (TailRecursion.tailrec_earlyout
+    (HList.polymorphic_list.cons (list byte) (HList.polymorphic_list.cons (mem -> Prop) HList.polymorphic_list.nil))
+    ["buf";"num_bytes";"i";"read";"err"]
+    (fun v scratch R t m buf num_bytes_loop i read err => PrimitivePair.pair.mk (
+      word.unsigned err = 0 /\
+      word.unsigned i <= word.unsigned num_bytes /\
+      v = word.unsigned i /\
+      (bytes (word.add buf i) scratch * R) m /\
+      Z.of_nat (List.length scratch) = word.unsigned (word.sub num_bytes i) /\
       word.unsigned i mod 4 = word.unsigned num_bytes mod 4 /\
-      num_bytes_loop = num_bytes
-      (* (word.unsigned i < word.unsigned num_bytes + 4) *)
-      (* /\  word.unsigned i < num_bytes) *) )  (* precondition of every loop *)
-      (fun T M BUF NUM_BYTES I READ => exists SCRATCH,
-        (array scalar8 (word.of_Z 1) (word.add buf i) SCRATCH * R) M /\
-        List.length SCRATCH = List.length scratch /\
-        NUM_BYTES = num_bytes)) (* postcondition *)
-    (fun n m : Z => m < n <= word.unsigned num_bytes) (* well_founded relation *)
-    _ _ _ _ _ _ _);
+      num_bytes_loop = num_bytes)
+    (fun T M BUF NUM_BYTES I READ ERR =>
+       NUM_BYTES = num_bytes_loop /\
+       exists RECV,
+       (bytes (word.add buf i) RECV * R) M /\
+       List.length RECV = List.length scratch /\
+       exists iol, T = iol ++ t /\
+       exists ioh, mmio_trace_abstraction_relation ioh iol /\
+       (word.unsigned ERR = 0 /\ lan9250_readpacket _ _ RECV ioh \/
+        word.unsigned ERR = 2^32-1 /\ TracePredicate.concat TracePredicate.any (spi_timeout word) ioh ) )
+    )
+    _ _ _ _ _ _ _ _);
   (* TODO wrap this into a tactic with the previous refine? *)
   cbn [HList.hlist.foralls HList.tuple.foralls
        HList.hlist.existss HList.tuple.existss
@@ -243,191 +358,256 @@ Proof.
        List.repeat Datatypes.length
        HList.polymorphic_list.repeat HList.polymorphic_list.length
        PrimitivePair.pair._1 PrimitivePair.pair._2] in *;
-  repeat (straightline || straightline_if || eapply interact_nomem || eauto 99).
-  { exact (Z.gt_wf _). }
-  { repeat (refine (conj _ _)); eauto.
-    { replace (word.add p_addr i) with p_addr by (subst i; ring).
-      rewrite <- (List.firstn_skipn (Z.to_nat (word.unsigned (word.sub num_bytes i) ) )  _) in H.
-      SeparationLogic.seprewrite_in (symmetry! @bytearray_index_merge) H; [|ecancel_assumption].
-      rewrite List.length_firstn_inbounds, ?Znat.Z2Nat.id; trivial.
-      { eapply Properties.word.unsigned_range. }
-      trans_ltu. eapply Znat.Nat2Z.inj_le. rewrite -> ?Znat.Z2Nat.id.
-      { rewrite -> H0.
-        replace (word.sub num_bytes i) with num_bytes by (subst i; ring).
-        rewrite word.unsigned_of_Z in H2. change (word.wrap 1521) with (1521) in H2.
-        Lia.lia. }
-      replace (word.sub num_bytes i) with num_bytes by (subst i; ring).
-      eapply Properties.word.unsigned_range. }
-    { replace (word.sub num_bytes i) with num_bytes by (subst i; ring).
-      rewrite -> List.length_firstn_inbounds.
-      { rewrite ?Znat.Z2Nat.id; trivial; eapply Properties.word.unsigned_range. }
-      rewrite H0. trans_ltu.
-      change (word.unsigned (word.of_Z 1521)) with (1521) in H2.
-      pose proof Properties.word.unsigned_range num_bytes.
-      PreOmega.zify.
-      rewrite ?Znat.Z2Nat.id; Lia.lia. }
-    { pose proof Properties.word.unsigned_range num_bytes. PreOmega.zify.
-      subst i. subst num_bytes. subst num_bytes2.
-      replace (word.add (word.add num_bytes1 num_bytes1) (word.add num_bytes1 num_bytes1)) with (word.mul num_bytes1 (word.of_Z 4)) in * by ring.
-      { rewrite word.unsigned_mul. unfold word.wrap.
-        rewrite (Z.mod_small _ (2^width)).
-        { change (word.unsigned (word.of_Z 0) mod 4) with 0.
-          change (word.unsigned (word.of_Z 4)) with 4.
-          Z.div_mod_to_equations.
-          Lia.lia. }
-        change (word.unsigned (word.of_Z 4)) with 4. subst num_bytes1.
-        rewrite Properties.word.unsigned_sru_nowrap.
-        { rewrite Z.shiftr_div_pow2.
-          { change (2 ^ word.unsigned (word.of_Z 2)) with 4.
-            pose proof Properties.word.unsigned_range (word.add num_bytes0 (word.of_Z 3)).
-            Z.div_mod_to_equations.
-            (*  0 <= word.unsigned num_words * word.unsigned (word.of_Z 4)
-                < 2 ^ width *)
-            Lia.lia. }
-          { cbv. congruence. }}
-        exact eq_refl. }}}
-    { straightline_call.
-      1: cbv - [Z.le Z.lt]; clear; blia.
-      repeat (straightline || straightline_if).
+    repeat (straightline || split_if || eapply interact_nomem || eauto 99).
+  { exact (Z.gt_wf (word.unsigned num_bytes)). }
+  1: repeat (refine (conj _ _)); eauto.
+  { eapply Properties.word.unsigned_range. }
+  1: zify_unsigned.
+  1: replace (word.add p_addr i) with p_addr by (subst i; ring).
+  1: rewrite <- (List.firstn_skipn (Z.to_nat (word.unsigned (word.sub num_bytes i) ) )  _) in H.
+  1: SeparationLogic.seprewrite_in (symmetry! @bytearray_index_merge) H; [|ecancel_assumption].
+    1,2,3:
+    repeat match goal with
+    | |- ?x = ?x => exact (eq_refl x)
+    | _ => progress trans_ltu
+    | _ => progress zify_unsigned
+    | _ => progress PreOmega.zify
+    | _ => progress rewrite ?Znat.Z2Nat.id by blia
+    | H: _ |- _ => progress (rewrite ?Znat.Z2Nat.id in H by blia)
+    | _ => rewrite List.length_firstn_inbounds by (PreOmega.zify; rewrite ?Znat.Z2Nat.id by blia; blia)
+    | _ => progress rewrite ?Z.sub_0_r
+    end; repeat straightline.
+    { repeat match goal with x:= _ |- context[?x]  => subst x end. clear. Z.div_mod_to_equations. blia. }
+
+    { straightline_call; repeat straightline.
+      { cbv; clear; intuition congruence. }
+      split_if; do 6 straightline.
+
+      (* SPI timeout, break loop *)
+      { straightline.
+        straightline.
+        straightline.
+        straightline.
+        (* [repeat straightline] hangs *)
+        do 5 eexists; split; [repeat straightline|]; [].
+        left.
+        repeat straightline.
+        { subst br0. rewrite word.unsigned_ltu, Z.ltb_irrefl; exact eq_refl. }
+        split; eauto.
+        eexists; split; eauto.
+        split; eauto.
+        eexists; split.
+        { subst a; eauto. }
+        eexists; split; eauto.
+        right; split.
+        { exact eq_refl. }
+        intuition eauto. }
+        
       (* store *)
-      do 2 trans_ltu. rewrite <- (List.firstn_skipn 4 _) in H4.
-      SeparationLogic.seprewrite_in (symmetry! @bytearray_index_merge) H4.
-      { rewrite List.length_firstn_inbounds.
-        { instantiate (1:= word.of_Z 4). eauto. }
-        apply Znat.Nat2Z.inj_le. rewrite H5. rewrite word.unsigned_sub.
-        unfold word.wrap. rewrite Z.mod_small.
-        { revert H6 H3. clear. Z.div_mod_to_equations.
-          (* Z.of_nat 4 <= word.unsigned x6 - word.unsigned x5 *)
-          Lia.lia. }
-        pose proof Properties.word.unsigned_range x4.
-        pose proof Properties.word.unsigned_range x5.
-        Lia.lia. } 
-      eapply store_four_of_sep.
-      { seprewrite_in @scalar32_of_bytes H8; [..|ecancel_assumption].
-        { exact _. }
-        { eapply List.length_firstn_inbounds. apply Znat.Nat2Z.inj_le. rewrite H5.
-          rewrite word.unsigned_sub. unfold word.wrap. rewrite Z.mod_small.
-          { revert H6 H3. clear. Z.div_mod_to_equations.
-            (* Z.of_nat 4 <= word.unsigned x6 - word.unsigned x5 *)
-            Lia.lia. }
-          pose proof Properties.word.unsigned_range x4.
-          pose proof Properties.word.unsigned_range x5.
-          (* 0 <= word.unsigned x6 - word.unsigned x5 < 2 ^ width *)
-          Lia.lia. }}
       do 4 straightline.
+      trans_ltu.
+      match goal with
+        | H: context[word.unsigned (word.sub ?a ?b)] |- _ =>
+            pose proof Properties.word.unsigned_range a;
+            pose proof Properties.word.unsigned_range b;
+            let H := fresh in
+            pose proof word.unsigned_sub a b as H;
+            unfold word.wrap in H;
+            rewrite Z.mod_small in H by blia
+      end.
+      match goal with H10 : _ ?a0 |- store _ ?a0 _ _ _ => rewrite <- (List.firstn_skipn 4 _) in H10;
+        SeparationLogic.seprewrite_in (symmetry! @bytearray_index_merge) H10 end.
+      { instantiate (1:= word.of_Z 4). rewrite List.length_firstn_inbounds; [exact eq_refl|]. Z.div_mod_to_equations. blia. }
+      eapply store_four_of_sep.
+      { match goal with H8:_|-_ => seprewrite_in @scalar32_of_bytes H8; [..|ecancel_assumption]; try exact _; [] end.
+        eapply List.length_firstn_inbounds; Z.div_mod_to_equations; blia. }
+
+      (* after store *)
+      do 5 straightline.
       (* TODO straightline hangs in TailRecursion.enforce *)
-      do 4 letexists. split. { repeat straightline. } do 3 letexists.
+      do 5 letexists. split. { repeat straightline. }
+      right. do 3 letexists.
       repeat split; repeat straightline; repeat split.
-      { replace (word.add x3 i)
-          with (word.add (word.add x3 x5) (word.of_Z 4)) by (subst i; ring).
+      { intuition idtac. }
+      { subst i.
+        rewrite word.unsigned_add; cbv [word.wrap]; rewrite Z.mod_small;
+        change (word.unsigned (word.of_Z 4)) with 4; try (Z.div_mod_to_equations; blia). }
+      { replace (word.add x9 i)
+          with (word.add (word.add x9 x11) (word.of_Z 4)) by (subst i; ring).
         ecancel_assumption. }
-      { subst x12. rewrite List.length_skipn. rewrite Znat.Nat2Z.inj_sub.
-        { rewrite H5. subst i.
-          replace (word.sub x4 (word.add x5 (word.of_Z 4)))
-            with (word.sub (word.sub x4 x5) (word.of_Z 4)) by ring.
+      { repeat match goal with x1 := _ |- _ => subst x1; rewrite List.length_skipn; rewrite Znat.Nat2Z.inj_sub end.
+        { repeat match goal with H5:_|-_=>rewrite H5 end; subst i.
+          progress replace (word.sub num_bytes (word.add x11 (word.of_Z 4)))
+            with (word.sub (word.sub num_bytes x11) (word.of_Z 4)) by ring.
           rewrite (word.unsigned_sub _ (word.of_Z 4)).
           unfold word.wrap. rewrite Z.mod_small.
-          { exact eq_refl. }
-          { change (word.unsigned (word.of_Z 4)) with 4.
-            pose proof Properties.word.unsigned_range (word.sub x3 x4).
-            pose proof Properties.word.unsigned_range x4.
-            pose proof Properties.word.unsigned_range x5.
-            rewrite word.unsigned_sub. unfold word.wrap. rewrite Z.mod_small.
-            { revert H10 H9 H7 H6 H3 H2. clear.
-              Z.div_mod_to_equations. Lia.lia. }
-            { Z.div_mod_to_equations. Lia.lia. }}}
-        apply Znat.Nat2Z.inj_le. rewrite H5. rewrite word.unsigned_sub.
-        unfold word.wrap. rewrite Z.mod_small.
-        { revert H6 H3. clear. Z.div_mod_to_equations. Lia.lia. }
-        pose proof Properties.word.unsigned_range x4.
-        pose proof Properties.word.unsigned_range x5.
-        Lia.lia. }
-      { subst i. rewrite word.unsigned_add. unfold word.wrap. rewrite (Z.mod_small _ (2 ^ width)).
-        { revert H6. clear. change (word.unsigned (word.of_Z 4)) with 4.
-          Z.div_mod_to_equations. Lia.lia. }
-        pose proof Properties.word.unsigned_range x4.
-        pose proof Properties.word.unsigned_range x5.
+          all: change (word.unsigned (word.of_Z 4)) with 4; change (Z.of_nat 4) with 4.
+          all : Z.div_mod_to_equations; blia. }
+        Z.div_mod_to_equations; blia. }
+      { subst i.
+        rewrite word.unsigned_add. unfold word.wrap. rewrite (Z.mod_small _ (2 ^ width)).
+        { revert dependent x11. clear. change (word.unsigned (word.of_Z 4)) with 4. intros.
+          Z.div_mod_to_equations. blia. }
         change (word.unsigned (word.of_Z 4)) with 4.
-        change (word.unsigned (word.of_Z 1521)) with 1521 in *.
-        revert H9 H7 H6 H3 H2. clear.
-        PreOmega.zify. Z.div_mod_to_equations. Lia.lia. }
+        Z.div_mod_to_equations.
+        blia. }
       { repeat match goal with |- context [?x] => is_var x; subst x end.
         rewrite word.unsigned_add. unfold word.wrap. rewrite Z.mod_small.
-        { change (word.unsigned (word.of_Z 4)) with 4. Lia.lia. }
-        pose proof Properties.word.unsigned_range x4.
-        pose proof Properties.word.unsigned_range x5.
-        change (word.unsigned (word.of_Z 4)) with 4.
-        change (word.unsigned (word.of_Z 1521)) with 1521 in *.
-        revert H9 H7 H6 H3 H2. clear.
-        PreOmega.zify. Z.div_mod_to_equations. Lia.lia. }
+        { change (word.unsigned (word.of_Z 4)) with 4. blia. }
+        change (word.unsigned (word.of_Z 4)) with 4. Z.div_mod_to_equations. blia. }
       { subst v'. subst i.
         rewrite word.unsigned_add. change (word.unsigned (word.of_Z 4)) with 4.
-        unfold word.wrap. rewrite (Z.mod_small _ (2 ^ width)).
-        { revert H6 H3. clear. Z.div_mod_to_equations. Lia.lia. }
-        { pose proof Properties.word.unsigned_range x4.
-          pose proof Properties.word.unsigned_range x5.
-          change (word.unsigned (word.of_Z 1521)) with 1521 in *.
-          PreOmega.zify. Z.div_mod_to_equations. Lia.lia. }}
-      { letexists. split.
-        { subst x12. subst i.
-          repeat match type of H7 with context [?x] => subst x end.
-          cbv [scalar32 truncated_scalar littleendian ptsto_bytes.ptsto_bytes] in H7.
-          replace (word.add x3 (word.add x5 (word.of_Z 4))) with
-                  (word.add (word.add x3 x5) (word.of_Z 4)) in H7 by ring.
-          SeparationLogic.seprewrite_in (@bytearray_index_merge) H7.
-          { exact eq_refl. } { ecancel_assumption. }}
-        split.
-        { subst SCRATCH. rewrite List.app_length. rewrite H9. subst x12. rewrite List.length_skipn.
-          change (Datatypes.length (HList.tuple.to_list (LittleEndian.split (bytes_per access_size.four) (word.unsigned (word.of_Z (word.unsigned x7)))))) with (4%nat).
-          assert (4 <= (Datatypes.length x1))%nat. 2:Lia.lia.
+        unfold word.wrap. rewrite (Z.mod_small _ (2 ^ width));
+          change (2^width) with (2^32) in *; Z.div_mod_to_equations; blia. }
+
+      { letexists; repeat split.
+        { repeat match goal with x := _ |- _ => is_var x; subst x end; subst.
+          cbv [scalar32 truncated_scalar littleendian ptsto_bytes.ptsto_bytes] in *.
+          progress replace (word.add x9 (word.add x11 (word.of_Z 4))) with
+                  (word.add (word.add x9 x11) (word.of_Z 4)) in * by ring.
+          SeparationLogic.seprewrite_in (@bytearray_index_merge) H25.
+          { exact eq_refl. } { ecancel_assumption. } }
+        { subst RECV. rewrite List.app_length.
+          rewrite H26. subst x22. rewrite List.length_skipn.
+          unshelve erewrite (_ : length (HList.tuple.to_list _) = 4%nat); [exact eq_refl|].
+          enough ((4 <= length x7)%nat) by blia.
+          Z.div_mod_to_equations; blia. }
+        repeat match goal with x := _ |- _ => is_var x; subst x end; subst.
+        eexists; split.
+        { rewrite List.app_assoc; eauto. }
+        eexists; split.
+        { eapply List.Forall2_app; eauto.  }
+        destruct H29; [left|right]; repeat (straightline || split || eauto using TracePredicate__any_app_more).
+        eapply TracePredicate.concat_app; eauto.
+        unshelve erewrite (_ : LittleEndian.combine _ _ = word.unsigned x10); rewrite !word.of_Z_unsigned; try solve [intuition idtac].
+        1: replace (word.unsigned x10) with (word.unsigned x10 mod 2^(Z.of_nat (bytes_per (width:=32) access_size.four)*8)).
+        1:rewrite <-LittleEndian.combine_split; f_equal.
+        eapply Properties.word.wrap_unsigned. } }
+
+    { split; eauto. eexists; split; eauto. split; eauto. exists nil; split; eauto.
+      eexists; split; [constructor|].
+      left. split; eauto.
+      enough (Hlen : length x7 = 0%nat) by (destruct x7; try solve[inversion Hlen]; exact eq_refl).
+      PreOmega.zify.
+      rewrite H13.
+      subst br.
+      rewrite word.unsigned_ltu in H11.
+      destruct (word.unsigned x11 <? word.unsigned num_bytes) eqn:HJ; try solve [inversion H11].
+      eapply Z.ltb_nlt in HJ.
+      revert dependent x7; revert dependent num_bytes; revert dependent x11; clear; intros.
+      unshelve erewrite (_:x11 = num_bytes) in *.
+      { eapply Properties.word.unsigned_inj. Z.div_mod_to_equations; Lia.lia. }
+      rewrite word.unsigned_sub, Z.sub_diag; exact eq_refl. }
+    repeat straightline.
+    repeat letexists. split. { repeat straightline. }
+    eexists _, _. split. { exact eq_refl. }
+
+    repeat straightline.
+    subst i.
+    match goal with H: _ |- _ =>
+      progress repeat (unshelve erewrite (_ : forall x, word.add x (word.of_Z 0) = x) in H; [intros; ring|]);
+      progress repeat (unshelve erewrite (_ : forall x, word.sub x (word.of_Z 0) = x) in H; [intros; ring|])
+    end.
+    eexists; split.
+    1: { repeat match goal with |- context [?x] => match type of x with list _ => subst x end end.
+      repeat rewrite List.app_assoc. f_equal. }
+    eexists; split.
+    1:repeat eapply List.Forall2_app; eauto.
+    destruct H14; [left|right]; repeat straightline; repeat split; eauto.
+    { trans_ltu; change (word.unsigned (word.of_Z 1521)) with 1521 in *; eexists _, _; repeat split.
+      { SeparationLogic.ecancel_assumption. }
+      { revert dependent x2. revert dependent x6. intros.
+        destruct H5; repeat straightline; try contradiction.
+        destruct H9; repeat straightline; try contradiction.
+        eexists _, _; split.
+        { rewrite <-!List.app_assoc. eauto using concat_app. }
+        split; [zify_unsigned; eauto|].
+      { cbv beta delta [lan9250_decode_length].
+        rewrite H11. rewrite List.firstn_length, Znat.Nat2Z.inj_min.
+        replace (word.sub num_bytes (word.of_Z 0)) with num_bytes by ring.
+        rewrite ?Znat.Z2Nat.id by eapply word.unsigned_range.
+        transitivity (word.unsigned num_bytes); [blia|exact eq_refl]. } }
+      { pose proof word.unsigned_range num_bytes.
+        rewrite length_skipn.
+        PreOmega.zify. rewrite ?Znat.Z2Nat.id in * by blia; blia. }
+      rewrite H11, length_firstn_inbounds, ?Znat.Z2Nat.id.
+      all : try (zify_unsigned;
+      try Lia.lia;
+      eapply Znat.Nat2Z.inj_le;
+      rewrite ?Znat.Z2Nat.id; Lia.lia).
+      }
+    { repeat match goal with H : _ |- _ => rewrite H; intro HX; solve[inversion HX] end. }
+    { trans_ltu; change (word.unsigned (word.of_Z 1521)) with 1521 in *.
+      eexists _; split; eauto; repeat split; try Lia.lia.
+      { SeparationLogic.seprewrite_in @bytearray_index_merge H10.
+        { rewrite H11.
+          1: replace (word.sub num_bytes (word.of_Z 0)) with num_bytes by ring.
+          rewrite List.length_firstn_inbounds, ?Znat.Z2Nat.id.
+          1:exact eq_refl.
+          1:eapply word.unsigned_range.
           PreOmega.zify.
-          rewrite H5. rewrite word.unsigned_sub. unfold word.wrap. rewrite (Z.mod_small _ (2 ^ width)).
-          { revert H6 H3. clear. change (word.unsigned (word.of_Z 4)) with 4.
-            Z.div_mod_to_equations. Lia.lia. }
-          pose proof Properties.word.unsigned_range x15.
-          pose proof Properties.word.unsigned_range x5.
-          Lia.lia. }
-        { reflexivity. }}}
-    { left. letexists. split. { repeat straightline. exact eq_refl. }
-      letexists. split.
-      { subst bytes_written. subst i.
-        replace (word.add p_addr (word.of_Z 0)) with (p_addr) in H3 by ring.
-        replace (word.add p_addr (word.sub x2 (word.of_Z 0)))
-          with (word.add p_addr x2) in H3 by ring.
-        replace (word.sub x2 (word.of_Z 0)) with (x2) in H3 by ring.
-        ecancel_assumption. }
-      subst bytes_written. subst rx_packet'. subst i. rewrite H4.
-      replace (word.sub x2 (word.of_Z 0)) with (x2) by ring.
-      rewrite List.length_firstn_inbounds, Znat.Z2Nat.id; trivial.
-      { reflexivity. }
-      { pose proof Properties.word.unsigned_range x2. apply H5. }
-      { rewrite H0.
-        pose proof Properties.word.unsigned_range x2.
-        trans_ltu. eapply Znat.Nat2Z.inj_le. rewrite -> Znat.Z2Nat.id.
-        { rewrite word.unsigned_of_Z in H2. change (word.wrap 1521) with (1521) in H2. Lia.lia. }
-        { eapply Properties.word.unsigned_range. }
-    }}
-    Grab Existential Variables. exact _.
-Qed.
+          rewrite ?Znat.Z2Nat.id by eapply word.unsigned_range.
+          blia. }
+        eapply H15. }
+      { 1:rewrite List.app_length, List.length_skipn, H11, List.firstn_length.
+        replace (word.sub num_bytes (word.of_Z 0)) with num_bytes by ring.
+        enough (Z.to_nat (word.unsigned num_bytes) <= length buf)%nat by blia.
+        PreOmega.zify. rewrite ?Znat.Z2Nat.id by eapply word.unsigned_range; blia. }
+      right. right. split; eauto using TracePredicate__any_app_more. } }
 
-Lemma lightbulb_ok : program_logic_goal_for_function! lightbulb.
-Proof.
-  repeat (eauto || straightline || straightline_if || eapply interact_nomem || prove_ext_spec).
 
-  trans_ltu.
-  repeat match goal with x := _ |- _ => subst x end.
-  rewrite word__unsigned_of_Z_nowrap in * by (change (2^width) with (2^32); blia).
+  all: repeat letexists; split; repeat straightline;
+    eexists _, _; split; [ exact eq_refl | ].
+  all: eexists; split;
+    [repeat match goal with |- context [?x] => match type of x with list _ => subst x end end;
+    rewrite ?List.app_assoc; eauto|].
+  all: eexists; split;
+    [repeat eapply List.Forall2_app; eauto|].
+  all:
+    right; subst err;
+    split; [intro HX; inversion HX|].
+  all : repeat ((eexists; split; [solve[eauto]|]) || (split; [solve[eauto]|])).
 
-  seplog_use_array_load1 H 12.
-  seplog_use_array_load1 H 13.
-  seplog_use_array_load1 H 23.
-  seplog_use_array_load1 H 42.
-  repeat (eauto || straightline || straightline_if || eapply interact_nomem || prove_ext_spec).
-Qed.
+  (* two cases of SPI timeout *)
+  { left; split; [exact eq_refl|] || right.
+    left; split; [exact eq_refl|] || right.
+          split; [exact eq_refl|].
+      intuition eauto using TracePredicate__any_app_more. }
+  { left; split; [exact eq_refl|] || right.
+    left; split; [exact eq_refl|] || right.
+          split; [exact eq_refl|].
+      intuition eauto using TracePredicate__any_app_more. }
+  { left; split; [exact eq_refl|] || right.
+    left; split; [exact eq_refl|].
+    eexists _, _; split.
+    1:eapply TracePredicate.concat_app; try intuition eassumption.
+    subst v0.
+    rewrite word.unsigned_ltu in H6.
+    destruct (word.unsigned num_bytes <? word.unsigned (word.of_Z 1521)) eqn:?; try inversion H6.
+    eapply Z.ltb_nlt in Heqb; revert Heqb.
+    repeat match goal with |- context [?x] => match type of x with _ => subst x end end.
+    cbv [lan9250_decode_length]. split. 2: cbn in *; blia.
+    subst v. rewrite word.unsigned_and_nowrap in H2. eapply H2. }
+  { left.
+    split; [exact eq_refl|].
+    eexists; split; intuition eauto. }
 
+  Unshelve.
+  exact _.
+Defined.
+
+(*
+Definition x := (iot_ok , lightbulb_ok , recvEthernet_ok , lan9250_readword_ok , spi_read_ok , spi_write_ok).
+Print Assumptions x.
+Axioms:, SortedListString.string_strict_order, TailRecursion.putmany_gather, parameters_ok FE310CSemantics.parameters, SortedList.TODO
+*)
+
+(*
 From bedrock2 Require Import ToCString Byte Bytedump.
 Local Open Scope bytedump_scope.
 Goal True.
+(* FIXME: name clashes between this file and lan9250_spec *)
   let c_code := eval cbv in (of_string (@c_module BasicCSyntax.to_c_parameters [iot; lightbulb; recvEthernet; lan9250_readword; spi_read; spi_write])) in
-  idtac c_code.
+  idtac (* c_code *).
 Abort.
+*)
